theories/ILL/IMSELL_undec.v
@@ -15,19 +15,27 @@ From Undecidability.CounterMachines
 From Undecidability.ILL
   Require Import IMSELL ndMM2_IMSELL.
 
+Local Infix "≤" := (@IMSELL_le _) (at level 70).
+Local Notation "u ≰ v" := (~ u ≤ v) (at level 70).
+Local Notation U := (@IMSELL_U _).
+
 (* Undecidability of IMSELL3, ie IMSELL with
    3 modalities {a,b,∞} with a,b < ∞ and 
    ∞ is the only universal modality *)
 
-Theorem IMSELL3_undec : undecidable (@IMSELL_cf_provable imsell3).
+Theorem IMSELL_undec (S : IMSELL_sig) : 
+     (exists a b i : S, a ≤ i /\ b ≤ i /\ a ≰ b /\ b ≰ a /\ ~ U a /\ ~ U b /\ U i)
+  -> undecidable (@IMSELL_cf_PROVABILITY S).
 Proof.
+  intro. 
   apply (undecidability_from_reducibility ndMM2_undec).
-  apply ndMM2_IMSELL.reduction.
+  now apply ndMM2_IMSELL.reduction.
 Qed.
 
-
-
-
-    
+Theorem IMSELL3_undec : undecidable (@IMSELL_cf_PROVABILITY imsell3).
+Proof.
+  apply IMSELL_undec.
+  now exists (Some true), (Some false), None.
+Qed.
 
 
